formalism: unify addresses representation
This patch unifies the model of an hardware address and an physical
address. The Address type gets a new component which identifies the
address space we are considering.

src/Address/PhysicalAddress_def.v
@@ -1,3 +1,0 @@
-Require Import SpecCert.Address.Address_ind.
-
-Definition PhysicalAddress := Address.
