src/Address.v
@@ -1,12 +1,4 @@
-Require Export SpecCert.Address.Address_ind.
-Require Export SpecCert.Address.Address_eq.
-Require Export SpecCert.Address.Address_proofs.
-Require Export SpecCert.Address.PhysicalAddress_def.
-Require Export SpecCert.Address.PhysicalAddress_prop.
-Require Export SpecCert.Address.PhysicalAddress_dec.
-Require Export SpecCert.Address.HardwareAddress_ind.
-Require Export SpecCert.Address.HardwareAddress_eq.
-Require Export SpecCert.Address.HardwareAddress_prop.
-Require Export SpecCert.Address.HardwareAddress_dec.
-Require Export SpecCert.Address.HardwareAddress_func.
 Require Export SpecCert.Address.AddressSpace.
+Require Export SpecCert.Address.Address.
+Require Export SpecCert.Address.PhysicalAddress.
+Require Export SpecCert.Address.HardwareAddress.
