src/Address/Address.v
@@ -1,0 +1,116 @@
+Require Import Coq.Arith.EqNat.
+Require Import Coq.Structures.DecidableType.
+Require Import Coq.Classes.EquivDec.
+Require Import Coq.Bool.Sumbool.
+
+Require Import SpecCert.Interval.
+Require Import SpecCert.Address.AddressSpace.
+Require Import SpecCert.Utils.
+
+(**
+Definitions
+ *)
+
+Inductive Address
+          (T: Type)
+  : Type :=
+| address (t: T)
+          (n:nat)
+          (h: is_inside_interval n address_space)
+  : Address T.
+
+Arguments address [T] (t n h).
+
+Definition address_offset
+           {T: Type}
+           (a:Address T) :=
+  match a with
+  | address _ x _ => x
+  end.
+
+Definition address_scope
+           {T: Type}
+           (a: Address T)
+  : T :=
+  match a with
+  | address t _ _ => t
+  end.
+
+(**
+   Equality
+ *)
+
+Definition addr_eq
+           {T: Type}
+           (a a':Address T) :=
+  address_offset a = address_offset a'
+  /\ address_scope a = address_scope a'.
+
+Axiom addr_eq_eq: forall {T: Type} (a a':Address T),
+    addr_eq a a' -> a = a'.
+Axiom eq_addr_eq: forall {T: Type} (a a': Address T),
+    a = a' -> addr_eq a a'.
+
+Lemma addr_eq_refl
+      {T: Type}
+  : forall (a: Address T), addr_eq a a.
+Proof.
+  intros a.
+  unfold addr_eq.
+  split; reflexivity.
+Qed.
+
+Lemma addr_eq_trans
+      {T :Type}
+  : forall (a a' a'':Address T),
+    addr_eq a a' -> addr_eq a' a'' -> addr_eq a a''.
+Proof.
+  intros a a' a'' [Ha1 Ha2] [Ha1' Ha2'].
+  unfold addr_eq in *.
+  rewrite <- Ha1'; rewrite <- Ha2'; rewrite <- Ha1; rewrite <- Ha2.
+  split; reflexivity.
+Qed.
+
+Lemma addr_eq_sym
+      {T: Type}
+  : forall (a a':Address T),
+    addr_eq a a' -> addr_eq a' a.
+Proof.
+  unfold addr_eq in *.
+  intros a a' [Heq Heq'].
+  rewrite Heq; rewrite Heq'.
+  split; reflexivity.
+Qed.
+
+Definition addr_eq_dec
+           {T:    Type}
+           (scope_eq_dec: forall (t t' :T), {t = t'}+{t <> t'})
+           (a a': Address T)
+  : {addr_eq a a'}+{~addr_eq a a'}.
+refine (
+    decide_dec (sumbool_and _
+                            _
+                            _
+                            _
+                            (eq_nat_decide (address_offset a) (address_offset a'))
+                            (scope_eq_dec (address_scope a) (address_scope a'))
+               )
+); unfold addr_eq; intuition.
+Defined.
+
+Parameters (T: Type)
+           (eqT: forall (t t': T), {t = t'}+{t <> t'}).
+
+Module Type Eq.
+  Parameter A: Type.
+  Parameter eq_dec: forall (a a': A), {a = a'}+{a <> a'}.
+End Eq.
+
+Module AddressDec (scope: Eq) <: DecidableType with Definition t := Address scope.A.
+  Definition t := Address scope.A.
+  Definition eq := @addr_eq scope.A.
+  Definition eq_refl := @addr_eq_refl scope.A.
+  Definition eq_sym := @addr_eq_sym scope.A.
+  Definition eq_trans := @addr_eq_trans scope.A.
+  Definition eq_dec := @addr_eq_dec scope.A scope.eq_dec.
+End AddressDec.
